examples/rel/IfcExampleReify3.fst
@@ -13,7 +13,7 @@ type env = id ->  Tot label
 type low_equiv (env:env) (h : rel heap)  =
   forall (x:id). {:pattern (Low? (env x))} (Low? (env x) ==> sel (R?.l h) x = sel (R?.r h) x)
 
-reifiable let p1 x y hi =
+ let p1 x y hi =
   begin if read hi = 0 then
     let vx = read x in
     let vy = read y in
