examples/rel/UnionFind.Forest.fst
@@ -30,13 +30,13 @@ let live (#n:nat) (uf:uf_forest n) (h:heap) :Type0 =
   (forall (i:id n).{:pattern (h `contains_a_well_typed` (index uf i))}
                h `contains_a_well_typed` (index uf i))  //all the refs in the forest are well typed
 
-reifiable let get (#n:nat) (uf:uf_forest n) (i:id n)
+ let get (#n:nat) (uf:uf_forest n) (i:id n)
   :ST (elt n) (requires (fun h0      -> live uf h0))
               (ensures  (fun h0 r h1 -> r == sel h0 (index uf i) /\ h0 == h1))
   = let h = STATE?.get () in
     sel_tot h (index uf i)
 
-reifiable let set (#n:nat) (uf:uf_forest n) (i:id n) (elt:elt n)
+ let set (#n:nat) (uf:uf_forest n) (i:id n) (elt:elt n)
   :ST unit (requires (fun h0      -> live uf h0))
            (ensures  (fun h0 _ h1 -> h1 == upd h0 (index uf i) elt))
   = let h0 = STATE?.get () in
